src/AsyncFinish/Typesystem.v
@@ -110,7 +110,7 @@ Inductive Typesystem (f:finish) (t:tid) : op -> Prop :=
   | check_end_finish:
     forall f',
     ~ Registered t f' -> (* the task executed its body *)
-    Child t (Blocked f') f ->
+    Child (t, (Blocked f')) f ->
     Typesystem f t END_FINISH.
 
 Inductive Check (f:finish) (t:tid) (o:op): Prop :=
